cp

coq/graph_model.v
@@ -4,9 +4,50 @@ Require Coq.Relations.Relation_Definitions.
 Require Import Lia.
 
 Require Export lc.tactics.
-Require Import lc.SetsAsPredicates.
 Require Import lc.AssocList.
 
+Require Import lc.SetsAsPredicates.
+Import SetNotations.
+Local Open Scope set_scope.
+
+Require Import Monad.
+Import MonadNotation.
+Open Scope monad_scope.
+
+(* stuff that should be in a library *)
+
+Inductive ExistsT {A : Type} (P : A -> Type) : list A -> Type :=
+  | ExistsT_cons1 : forall (x : A) (l : list A), 
+      P x  -> ExistsT P (x :: l)
+  | ExistsT_cons2 : forall (x : A) (l : list A), 
+      ExistsT P l -> ExistsT P (x :: l).
+
+Inductive Exists2 {A : Type} (P : A -> A -> Prop) : 
+  list A -> list A -> Prop :=
+    Exists2_cons_hd : forall (x y : A) (l l' : list A), 
+      P x y -> Exists2 P (x :: l) (y :: l')
+  | Exists2_cons_tl : forall (x y : A) (l l' : list A), 
+      Exists2 P l l' -> Exists2 P (x :: l) (y :: l').
+
+Hint Constructors ExistsT Exists2 : core.
+
+Lemma Forall_Forall2 {A} {P : A -> A -> Prop} l : 
+  Forall (fun x : A => P x x) l <->
+  Forall2 P l l.
+Proof.
+  induction l; split; intro h; inversion h; subst; eauto.
+  econstructor; eauto. rewrite <- IHl. auto.
+  econstructor; eauto. rewrite -> IHl. auto.
+Qed.
+
+Lemma Forall2_length {A} {P : A -> A -> Prop} l1 l2 : 
+  Forall2 P l1 l2 -> 
+  length l1 = length l2.
+Proof.
+  move: l2.
+  induction l1; intros l2 h;
+  inversion h; subst; simpl in *; eauto.
+Qed.  
 
 (* This a "Graph Model" of the CBV lambda calculus based on Jeremy Siek's Agda
    development.
@@ -15,6 +56,9 @@ Require Import lc.AssocList.
    is a set of its mappings. We need an infinite set to fully represent a
    function but any computation only requires a finite approximation of that 
    function.
+
+   This development extends Jeremy's language with (untyped) lists, numbers
+   (for accessing the lists by index) and 'wrong' for runtime type errors.
 
 *)
 
@@ -28,31 +72,392 @@ Require Import lc.AssocList.
    ⊆  \subseteq   (Included)
 *)
 
+(* ----------------------------------------------- *)
+
+(* Values *)
+
 Inductive Value : Type :=
-  | v_nat : nat -> Value 
-    (* one entry in a function's table *)
+  (* natural number *)
+  | v_nat : nat -> Value
+
+  (* one entry in a function's table *)
   | v_map : list Value -> Value -> Value
-    (* trivial function value, evaluated to a value but never applied *)
+
+  (* trivial function value, evaluated to a value but never applied *)
   | v_fun : Value
-    (* list/tuple of values *)
+
+  (* list/tuple of values *)
   | v_list : list Value -> Value
-    (* dynamic type error *)
+
+  (* dynamic type error *)
   | v_wrong : Value
 .
 
-(* ------------ Functions ------------------ *)
+(* 
+   The default induction principle for values is not
+   strong enough for lists in the v_map and v_list case. So we prove a stronger
+   version below.
 
-Infix "↦" := v_map (at level 85, right associativity).
+   Value_ind
+     : forall P : Value -> Prop,
+       (forall n : nat, P (v_nat n)) ->
+       (forall (l : list Value) (v : Value), P v -> P (v_map l v)) ->
+       P v_fun -> 
+       (forall l : list Value, P (v_list l)) -> 
+       P v_wrong -> 
+       forall v : Value, P v 
+*)
 
-Import SetNotations.
-Local Open Scope set_scope.
+Fixpoint Value_ind' (P : Value -> Prop)
+       (n : forall n : nat, P (v_nat n)) 
+       (m : forall (l : list Value) (v : Value), Forall P l -> P v -> P (v_map l v)) 
+       (f : P v_fun)
+       (l : (forall l : list Value, Forall P l -> P (v_list l)))
+       (w : P v_wrong) 
+       (v : Value) : P v := 
+  let rec := Value_ind' P n m f l w 
+  in
+  let fix rec_list (vs : list Value) : Forall P vs :=
+    match vs with 
+    | nil => Forall_nil _
+    | cons w ws => @Forall_cons Value P w ws (rec w) (rec_list ws)
+    end
+  in 
+  match v with 
+  | v_nat k => n k
+  | v_map X v => 
+      m X v (rec_list X) (rec v)
+  | v_fun => f
+  | v_list X => l X (rec_list X)
+  | v_wrong => w 
+  end.
 
-Definition Λ : (P Value -> P Value) -> P Value :=
-  fun f => fun v => match v with 
-          | (V ↦ w) => (w ∈ f (mem V)) /\ V <> nil /\ not (v_wrong ∈ mem V)
-          | v_fun => True
-          | _ => False
-          end.
+(* We do the same thing for Value_rect *)
+
+Inductive ForallT {A : Type} (P : A -> Type) : list A -> Type :=
+    ForallT_nil : ForallT P nil
+  | ForallT_cons : forall (x : A) (l : list A), P x -> ForallT P l -> ForallT P (x :: l).
+
+Fixpoint Value_rec' (P : Value -> Type)
+       (n : forall n : nat, P (v_nat n)) 
+       (m : forall (l : list Value) (v : Value),
+           ForallT P l -> P v -> P (v_map l v)) 
+       (f : P v_fun)
+       (l : (forall l : list Value, ForallT P l -> P (v_list l)))
+       (w : P v_wrong) (v : Value) : P v := 
+  let rec := Value_rec' P n m f l w 
+  in
+  let fix rec_list (vs : list Value) : ForallT P vs :=
+    match vs with 
+    | nil => ForallT_nil _
+    | cons w ws => @ForallT_cons Value P w ws (rec w) (rec_list ws)
+    end
+  in 
+  match v with 
+  | v_nat k => n k
+  | v_map X v => 
+      m X v (rec_list X) (rec v)
+  | v_fun => f
+  | v_list X => l X (rec_list X)
+  | v_wrong => w 
+  end.
+
+
+
+(* ----------------------------------------------- *)
+
+(* Consistent values: we will model function values as a set of approximations
+
+   But now that we have different sorts of values, those approximations should
+   all agree with eachother.
+
+   We can define this concept by first identifying the head of a value. 
+   Two values will *definitely* be inconsistent if they have different heads.
+   But they could have the same head if inside the value
+
+*)
+
+Inductive v_head := 
+   h_nat  : nat -> v_head 
+  | h_fun  : v_head
+  | h_list : v_head
+  | h_wrong : v_head 
+.
+
+Definition head (v : Value) : v_head := 
+  match v with 
+  | v_nat k => h_nat k
+  | v_map _ _ => h_fun
+  | v_fun => h_fun
+  | v_list _ => h_list
+  | v_wrong => h_wrong
+  end.
+
+
+Inductive Consistent : Value -> Value -> Prop :=
+  | c_nat : forall i, Consistent (v_nat i) (v_nat i)
+  | c_list : forall XS YS, Forall2 Consistent XS YS ->
+      Consistent (v_list XS) (v_list YS)
+  | c_wrong : Consistent v_wrong v_wrong
+
+  | c_fun : Consistent v_fun v_fun
+  | c_fun1 : forall X r, Consistent v_fun (v_map X r)
+  | c_fun2 : forall X r, Consistent (v_map X r) v_fun
+
+    (* maps that produce consistent results are consistent *)
+  | c_map2 : forall X1 X2 r1 r2,
+      Consistent r1 r2 -> 
+      Consistent (v_map X1 r1) (v_map X2 r2)
+
+    (* maps that don't overlap in their inputs are consistent *)
+    (* note: should this be exists or forall? *)
+  | c_map1 : forall X1 X2 r1 r2, 
+      (exists x1 x2, List.In x1 X1 /\ List.In x2 X2 /\ Inconsistent x1 x2) ->
+      Consistent (v_map X1 r1) (v_map X2 r2)
+
+with Inconsistent : Value -> Value -> Prop :=
+  | i_head : forall x y, 
+      head x <> head y ->
+      Inconsistent x y
+  | i_list_l : forall XS YS, 
+      length XS <> length YS ->
+      Inconsistent (v_list XS) (v_list YS)      
+  | i_list_e : forall XS YS,
+      Exists2 Inconsistent XS YS ->
+      Inconsistent (v_list XS) (v_list YS)
+  | i_map : forall X1 X2 r1 r2,
+      (forall x1 x2, List.In x1 X1 -> List.In x2 X2 -> Consistent x1 x2) ->
+      Inconsistent r1 r2 ->
+      Inconsistent (v_map X1 r1) (v_map X2 r2).
+
+Hint Constructors Consistent Inconsistent : core.
+
+(* There are two ways to compare lists of values for consistency:
+
+     Pointwise - corresponding elements must be consistent
+     Any - all pairs of elements from the two lists must be consistent
+
+ *)
+
+Definition ConsistentPointwiseList XS YS := 
+  Forall2 Consistent XS YS.
+Definition InconsistentPointwiseList XS YS := 
+  length XS <> length YS \/ Exists2 Inconsistent XS YS.
+Definition ConsistentAnyList XS YS := 
+  forall x y, List.In x XS -> List.In y YS -> Consistent x y.
+Definition InconsistentAnyList XS YS := 
+  (exists x y, List.In x XS /\ List.In y YS /\ Inconsistent x y).
+
+
+(* A set of values is consistent if all members are 
+   consistent with eachother *)
+Definition ConsistentSet := 
+  fun V : P Value => 
+    forall x y, x ∈ V -> y ∈ V -> Consistent x y.
+
+(* Two values cannot be both consistent and inconsistent. *)
+
+Lemma Consistent_Inconsistent_disjoint : 
+  forall x y, Consistent x y -> Inconsistent x y -> False.
+Proof.
+  intros x.
+  eapply Value_ind' with (P := fun x => 
+  forall y : Value, Consistent x y -> Inconsistent x y -> False).
+  all: intros.
+  all: try solve [inversion H; inversion H0; subst; done].
+  + inversion H2; inversion H1; subst.
+    all: try simpl in H3; try done.
+    - inversion H9; subst. clear H9.
+      eapply H0; eauto.
+    - inversion H9; subst. clear H9.
+    destruct H11 as [x1 [x2 [I1 [I2 ii]]]].
+    specialize (H5 _ _ I1 I2).
+    rewrite Forall_forall in H.
+    eapply H; eauto.
+  + inversion H0; inversion H1; subst. simpl in H5; try done.
+    - inversion H7; subst. eauto using Forall2_length.
+    - inversion H7; subst; clear H7.
+      clear H1 H0. move: YS H3 H6.
+      induction H; intros YS h1 h2;
+        inversion h1; inversion h2; subst.  
+      inversion H7; subst. eauto.
+      inversion H7; subst. eauto.
+Qed.
+
+(* Determining whether two values are consistent or inconsistent 
+   is decidable *)
+
+Definition ConsistentDecidable := fun v1 => forall v2 : Value, 
+                     {Consistent v1 v2} + {Inconsistent v1 v2}.
+
+
+
+Lemma dec_any : forall XS, ForallT ConsistentDecidable XS -> forall YS, { ConsistentAnyList XS YS } + {InconsistentAnyList XS YS}.
+induction XS.
+- intros h. intros ys. left. intros x y h1 h2. inversion h1.
+- intros h. inversion h. subst. clear h.
+  intros YS. unfold ConsistentDecidable in H1.
+  destruct (IHXS H2 YS).
+  + induction YS. left. intros x y h1 h2. inversion h2.
+    have CE: (ConsistentAnyList XS YS).
+    intros x y h1 h2. 
+    eapply c; eauto. simpl. eauto.
+    specialize (IHYS CE). destruct IHYS.
+    ++ destruct (H1 a0).       
+       left. 
+       { intros x y h1 h2.
+         destruct h1 as [EQ|INXS]; destruct h2 as [EQ2|INYS]; subst.
+         -- auto.
+         -- apply c0; eauto. simpl; auto.
+         -- apply c; eauto. simpl; auto.
+         -- apply CE; eauto.
+       } 
+       right. exists a . exists a0. simpl. split; auto.
+    ++ right. destruct i as [x [y [h1 [h2 h3]]]].
+       exists x. exists y. simpl. eauto.
+
+  + right. destruct i as [x1 [x2 [h1 [h2]]]].
+    exists x1. exists x2. simpl. split; eauto. 
+Qed.
+
+Lemma dec_point : forall XS,  ForallT ConsistentDecidable XS -> forall YS, { ConsistentPointwiseList XS YS } + {InconsistentPointwiseList XS YS}.
+Proof.  
+induction XS; intros IH [|y YS].
++ left. unfold ConsistentPointwiseList. eauto.
++ right. unfold InconsistentPointwiseList. simpl; left; auto.
++ right. left; simpl; auto.
++ inversion IH; subst. 
+  destruct (H1 y); destruct (IHXS H2 YS); unfold ConsistentPointwiseList in *; 
+    unfold InconsistentPointwiseList in *.
+  all: try solve [simpl; left; eauto].
+  all: try solve [right; destruct i; simpl; right; eauto].
+  right; destruct i; simpl. left; eauto. right; eauto.
+Qed.  
+  
+Lemma dec_con : forall v1 v2, {Consistent v1 v2 } + {Inconsistent v1 v2 }.
+intros v1. 
+eapply Value_rec' with 
+(P := fun v1 =>  forall v2 : Value, {Consistent v1 v2} + {Inconsistent v1 v2}).
+all: intros.
+all: destruct v2.
+all: try solve [right; eapply i_head; simpl; done].
+all: try solve [left; eauto].
++ destruct (Nat.eq_dec n n0). subst.
+  left. eauto. right. eapply i_head; simpl. intro h.
+  inversion h. subst.  done.
++ destruct (H0 v2).
+  left. eapply c_map2; eauto.
+  destruct (dec_any l H l0).
+  right. eapply i_map; eauto.
+  left. eauto.
++ destruct (dec_point l H l0).
+  left; eauto.
+  right. destruct i; eauto.
+Qed.
+
+(* Consistency is also reflexive *)
+
+Definition ConsistentReflexive (x : Value) := Consistent x x.
+
+Lemma ConsistentPointwiseList_refl : forall XS, ForallT ConsistentReflexive XS -> ConsistentPointwiseList XS XS. 
+Proof.
+  induction 1; unfold ConsistentPointwiseList; eauto.
+Qed.
+
+#[export] Instance Consistent_refl : Reflexive Consistent.
+intro x.
+eapply Value_ind' with (P := ConsistentReflexive).
+all: unfold ConsistentReflexive; intros; eauto using ConsistentPointwiseList_refl.
+econstructor. rewrite <- Forall_Forall2. auto.
+Qed.
+
+(* ------------------------------------------------- *)
+(* Consistent sets *)
+
+(*
+Section ConsistentSets.
+
+
+(* Can we restrict ⊆ so that consistent sets stay consistent? *)
+
+Definition IncludedConsistent (w1 w2 : P Value) := 
+  forall x : Value, 
+  (x ∈ w1 -> x ∈ w2) /\ (x ∈ w2 -> forall y, y ∈ w1 -> Consistent x y).
+
+Class CS (X : Type) := 
+  { consistent : X -> X -> Prop;
+    inconsistent : X -> X -> Prop;
+    exclusive : forall x y, consistent x y -> inconsistent x y -> False;
+    decidable : forall x y, { consistent x y } + { inconsistent x y };
+    reflexive : forall x, consistent x x
+  }.
+
+
+End ConsistentSets.
+*)
+
+(* Valid ---- -------------------------------------- *)
+
+(* A `P Value` is the denotation of an actual lambda-calculus value if it is
+   inhabited and does not contain wrong.
+*)
+
+Definition valid_witness (x : Value) (V : P Value) : Prop :=
+   (x ∈ V) /\ not (v_wrong ∈ V).
+
+Definition valid (V : P Value) : Type :=
+  { x : Value & valid_witness x V }.
+
+(* valid sets are inhabited *)
+Lemma valid_is_nonempty V : valid V -> nonemptyT V.
+  intros [x [P _]]. econstructor; eauto. Defined.
+
+(* A valid finite set: The witness is the first element in the list *)
+Definition valid_mem (V : list Value) : Prop :=
+  match V with 
+    | x :: _ => valid_witness x (mem V)
+    | _ => False
+  end.
+
+Lemma valid_mem_valid : forall V, valid_mem V -> valid (mem V).
+Proof.
+  intros V VM.
+  destruct V; simpl in *. done.
+  exists v. auto.
+Qed.
+
+#[export] Hint Immediate valid_mem_valid : core.
+
+Lemma wrong_not_valid : forall X, valid X -> not (v_wrong ∈ X).
+Proof.
+  intros X V h.
+  destruct V as [x [h0 h1]]. done.
+Qed.
+
+(* A finite, inhabited subset of a valid set is valid *)
+Lemma valid_sub_valid_mem {D a} : D <> nil -> valid a -> mem D ⊆ a -> valid_mem D.
+Proof.
+  intros NE V S.
+  inversion V.
+  unfold valid_mem.
+  unfold valid_witness in *.
+  destruct D. done.
+  move: H => [ii cc].
+  split; auto.
+Qed.
+
+Lemma valid_join : forall v1 v2, 
+    valid v1 -> 
+    valid v2 ->
+    valid (v1 ∪ v2).
+Proof.
+  intros v1 v2 [x1 [I1 h1]] [x2 [I2 h2]].
+  exists x1. unfold valid_witness. split.
+  eapply Union_introl; eauto.
+  intro h. inversion h; subst; done.
+Qed.
+
+(* ------------ Lists ------------------ *)
 
 Definition LIST : list (P Value) -> P Value  :=
   fun DS w => 
@@ -60,6 +465,47 @@ Definition LIST : list (P Value) -> P Value  :=
     | v_list WS => Forall2 In DS WS
     | _ => False
     end.
+
+Definition NIL : P Value := ⌈ v_list nil ⌉.
+
+Definition CONS : P Value -> P Value -> P Value := 
+  fun V W x => 
+    match x with 
+    | v_list (v :: w) => (v ∈ V) /\ (v_list w ∈ W)
+    | _ => False
+    end.
+        
+Lemma CONS_mono_sub { D1 D2 D3 D4 } :
+    D1 ⊆ D3 -> D2 ⊆ D4 -> ((CONS D1 D2) ⊆ (CONS D3 D4)).
+Proof.  
+  intros D13 D24 w C. 
+  unfold CONS, In in C.
+  destruct w; simpl in C; try done.
+  destruct l; try done.
+  move: C => [ d1 d2 ].
+  unfold CONS, In. split.
+  eapply D13; auto.
+  eapply D24; auto.
+Qed.
+
+Lemma CONS_cong { D1 D2 D3 D4 } :
+    D1 ≃ D3 -> D2 ≃ D4 -> ((CONS D1 D2) ≃ (CONS D3 D4)).
+Proof.
+  intros [ d13 d31 ] [ d24 d42 ].
+  split; eapply CONS_mono_sub; eauto.
+Qed.
+
+
+(* ------------ Functions ------------------ *)
+
+Infix "↦" := v_map (at level 85, right associativity).
+
+Definition Λ : (P Value -> P Value) -> P Value :=
+  fun f => fun v => match v with 
+          | (V ↦ w) => (w ∈ f (mem V)) /\ valid_mem V
+          | v_fun => True
+          | _ => False
+          end.
 
 (* 4 possibilities in application: 
    1. v_wrong e |-> v_wrong
@@ -77,16 +523,24 @@ Inductive APPLY : P Value -> P Value -> Value -> Prop :=
      (v_wrong ∈ D2) 
      -> APPLY D1 D2 v_wrong
   | BETA : forall D1 D2 w V,
-     (V ↦ w ∈ D1) -> (mem V ⊆ D2) -> V <> nil -> not (v_wrong ∈ mem V)
-     -> APPLY D1 D2 w
+     (V ↦ w ∈ D1) -> (mem V ⊆ D2) -> valid_mem V ->
+     APPLY D1 D2 w
   | PROJ   : forall D1 D2 w VS k, 
      (v_list VS ∈ D1) -> (v_nat k ∈ D2) -> nth_error VS k = Some w
      -> APPLY D1 D2 w.
 
+(*  < 1 , 2 > (\x.x)  --> wrong?? 
+
+    want to prove that we go wrong in enough places
+
+*)
+
+
+
 
 Infix "▩" := APPLY (at level 90).
 
-Definition den_nat : nat -> P Value :=
+Definition NAT : nat -> P Value :=
   fun j v => match v with 
           | v_nat k => j = k
           | _ => False
@@ -98,7 +552,7 @@ Definition den_nat : nat -> P Value :=
      <i,j> |-> i+j
      V |-> WRONG   where V /= <i,j>
 *)
-Definition den_add : P Value :=
+Definition ADD : P Value :=
   fun w => 
     match w with 
     | (V ↦ v_nat k) => 
@@ -112,16 +566,17 @@ Definition den_add : P Value :=
 (* -- Basic Properties of Denotational Operators --------------------------------- *) 
 
 (* k∈℘k *)
-Lemma k_in_den_k : forall k, v_nat k ∈ den_nat k.
+Lemma k_in_den_k : forall k, v_nat k ∈ NAT k.
 Proof. intros. reflexivity. Qed.
 
-Lemma k_in_den_k'_inv : forall k k', v_nat k ∈ den_nat k' -> k = k'.
+Lemma k_in_den_k'_inv : forall k k', v_nat k ∈ NAT k' -> k = k'.
 Proof. intros. inversion H. done. Qed.
 
-Lemma v_in_den_k_inv :  forall v k, v ∈ den_nat k -> v = v_nat k.
+Lemma v_in_den_k_inv :  forall v k, v ∈ NAT k -> v = v_nat k.
 Proof. intros. destruct v; inversion H. done. Qed.
 
 (*  Application is a Congruence ------------------------------------------------ *)
+                          
 
 Lemma APPLY_mono_sub { D1 D2 D3 D4 } :
     D1 ⊆ D3 -> D2 ⊆ D4 -> ((D1 ▩ D2) ⊆ (D3 ▩ D4)).
@@ -142,28 +597,26 @@ Proof.
   split; eapply APPLY_mono_sub; eauto.
 Qed.
 
-(* Valid ---- -------------------------------------- *)
 
-(* A `P Value` is the denotation of an actual lambda-calculus value if it is
-   an inhabited set that does not include wrong. We put this definition 
-   in `Type` so that we can extract the inhabitant. 
-*)
-
-Definition valid (V : P Value) : Type :=
-  { x : Value & ((x ∈ V) /\ not (v_wrong ∈ V)) }.
-
-Lemma valid_is_nonempty V : valid V -> nonemptyT V.
-  intros [x [P _]]. econstructor; eauto. Defined.
-
-(* Our meta-operators produce valid results. *)
+(* ---------- meta-operators produce valid results ------------------ *)
 
 Lemma valid_Λ : forall F, valid (Λ F).
 Proof. 
   intros F. unfold Λ, valid.
-  exists v_fun. split. cbv. auto. cbv.  auto.
+  exists v_fun. split. cbv. auto.
+  unfold In. done.
 Qed.
 
-#[export] Hint Resolve valid_Λ : core.
+ 
+Lemma valid_LIST : forall D, ForallT valid D -> valid (LIST D).
+induction 1; unfold LIST, valid, valid_witness, In. 
+exists (v_list nil). split; auto.
+destruct IHX as [xs [nin h]].
+destruct p as [y [niny hy]]. 
+Abort.
+
+
+(* #[export] Hint Resolve valid_Λ : core. *)
 
 (*  Abstraction is Extensional ---- -------------------------------------- *)
 
@@ -172,11 +625,7 @@ Lemma Λ_ext_sub {F1 F2} :
   (forall {X : P Value}, valid X -> F1 X ⊆ F2 X) -> Λ F1 ⊆ Λ F2.
 Proof.
   intros F1F2 v Iv. destruct v eqn:E; inversion Iv.
-  - move: H0 => [NN NW]. 
-    split. eapply F1F2; eauto. 
-    destruct l as [|w l]; try done. 
-    econstructor; eauto.
-    split. auto. auto.
+  - split; auto. eapply F1F2; eauto. 
   - trivial.
 Qed.
 
@@ -192,7 +641,7 @@ Qed.
 
 Definition continuous (F : P Value -> P Value) : Set :=
   forall X E, mem E ⊆ F X -> valid X 
-         -> exists D, (mem D ⊆ X) /\ ((mem E) ⊆ F (mem D)) /\ D <> nil.
+         -> exists D, (mem D ⊆ X) /\ ((mem E) ⊆ F (mem D)) /\ valid_mem D.
 
 Definition monotone (F : P Value -> P Value) : Set := 
   forall D1 D2, (D1 ⊆ D2) -> F D1 ⊆ F D2.
@@ -206,8 +655,9 @@ Proof.
   split.
   + intros w APP. inversion APP; subst. 
     - inversion H.
-    - move: NEX => [x [_ W]]. done.
-    - inversion H. eapply (Fmono (mem V) X); eauto. 
+    - exfalso. eapply wrong_not_valid; eauto. 
+    - inversion H.
+      eapply (Fmono (mem V) X); eauto. 
     - inversion H.
   + intros w wInFX.
     have M: mem (cons w nil) ⊆ F X. 
@@ -221,7 +671,7 @@ Qed.
 
 (*  Primitive Abstraction followed by Application is the identity --------- *)
 
-Lemma den_list : forall i j V, mem V ⊆ LIST (den_nat i :: den_nat j :: nil) ->
+Lemma den_list : forall i j V, mem V ⊆ LIST (NAT i :: NAT j :: nil) ->
                  forall x, x ∈ mem V -> x = v_list (v_nat i :: v_nat j :: nil).
 Proof.
   induction V.  intros. done.
@@ -237,14 +687,19 @@ Proof.
   auto.
 Qed.
 
-Lemma add_APPLY {i j} : 
-  den_add ▩ (LIST (den_nat i :: den_nat j :: nil)) ≃ den_nat (i + j).
+Lemma mem_one_inv : forall A (h v : A),  
+ h ∈ mem (v :: nil) -> h = v.
+Proof. 
+  intros. cbn in H. destruct H; try done.
+Qed. 
+
+Lemma ADD_APPLY {i j} : 
+  ADD ▩ (LIST (NAT i :: NAT j :: nil)) ≃ NAT (i + j).
 Proof.
   split.
   + intros w APP. inversion APP; subst; clear APP.
     all: cbn in H.
     all: try done.
-
     destruct w; try done.
     - destruct H as [i0 [j0 [h0 h1]]]. subst.
       move: (den_list _ _ _ H0 _ h0) => h1. inversion h1. subst. clear h1.
@@ -261,12 +716,8 @@ Proof.
      - intros x xIn. inversion xIn. subst.
        cbn. eauto using k_in_den_k.
        inversion H.
-     - intro h. done.
-     - intro h. cbn in h. destruct h as [v1 | v2]; try done.
+     - cbn. split. eauto. unfold In, mem. intro h. inversion h. done. done.
 Qed.
-
-(* This is about primitive functions, so skip for now *)
-
 
 (* Environments ---------------------- *)
 
@@ -330,6 +781,15 @@ Proof. unfold valid_env. eauto. Qed.
 
 #[export] Hint Resolve valid_nil : core.
 
+
+Lemma extend_valid_env {ρ x X} : 
+  x `notin` dom ρ ->
+  valid X -> 
+  valid_env ρ -> valid_env (x ~ X ++ ρ).
+Proof. intros Fr NEP NEX. eapply allT_cons; eauto. Qed.
+
+#[export] Hint Resolve extend_valid_env : core.
+
 (* A finite environment has a list of values for 
    each variable. *)
 
@@ -343,13 +803,136 @@ Lemma extend_nonempty_env {ρ x X} :
   nonempty_env ρ -> nonempty_env (x ~ X ++ ρ).
 Proof. intros Fr NEP NEX. eapply allT_cons; eauto. Qed.
 
-Lemma extend_valid_env {ρ x X} : 
-  x `notin` dom ρ ->
-  valid X -> 
-  valid_env ρ -> valid_env (x ~ X ++ ρ).
-Proof. intros Fr NEP NEX. eapply allT_cons; eauto. Qed.
+#[export] Hint Resolve extend_nonempty_env : core.
 
-#[export] Hint Resolve extend_nonempty_env extend_valid_env : core.
+
+(* A consistent finite value is one where all 
+   
+Definition Consistent_finite := fun V : P Value => 
+ forall E, (V ≃ mem E) -> ConsistentAnyList E E.
+
+Lemma disjoint_Consistent : forall x y, Consistent x y -> Inconsistent x y -> False.
+Admitted.
+*)
+
+Definition APPLY_Consistent : forall w1 w2, 
+    ConsistentSet w1 -> 
+    ConsistentSet w2 ->
+    ConsistentSet (APPLY w1 w2). 
+Proof.
+  intros w1 w2 C1 C2.
+  unfold ConsistentSet in *.
+  intros x y h1 h2. 
+  inversion h1; inversion h2; subst; eauto.
+  all: try (move: (C1 _ _ H H3) => h; inversion h; subst; auto).
+  all: try (move: (C2 _ _ H H4) => h; inversion h; subst; auto).
+  all: try (move: (C1 _ _ H H5) => h; inversion h; subst; auto).
+  all: try (move: (C2 _ _ H0 H5) => h; inversion h; subst; auto).
+
+  destruct V; try done.
+  move: H5 => [h3 h4]. 
+  have h5: v ∈ w2. eapply H4. eauto.
+  move: (C2 _ _ H h5) => Cwv.
+  inversion Cwv. subst.
+  assert False. eapply h4. eauto. done.
+
+  destruct V; try done.
+  move: H1 => [h3 h4]. 
+  have h5: v ∈ w2. eapply H0. eauto.
+  move: (C2 _ _ H5 h5) => Cwv.
+  inversion Cwv. subst.
+  assert False. eapply h4. eauto. done.
+
+  clear h.
+  move: H3 => [x1 [x2 [I1 [I2 ii]]]].
+  have h3 : x1 ∈ w2. eapply H0; eauto.
+  have h4 : x2 ∈ w2. eapply H6; eauto.
+  move: (C2 x1 x2 h3 h4) => h.
+  assert False. eapply Consistent_Inconsistent_disjoint; eauto. done.
+
+  move: (C2 _ _ H0 H6)=> c1. inversion c1; subst; clear c1; eauto. 
+  clear h1 h2 h H H0 H5 H6.
+  move: k0 H1 H7.
+  induction H4; intros k0; destruct k0; simpl;  try done.
+  + intros h1 h2; inversion h1; inversion h2; subst. auto.
+  + intros h1 h2. eauto.
+Qed.
+
+(*
+inversion h1'; subst; inversion h2'; subst; eauto.
+all: try solve [rewrite E1 in H; rewrite E1 in H0;
+  move: (C1 _ _ H H0) => h; inversion h].
+rewrite E2 in H. rewrite E2 in H1. admit. (* need to keep v_wrong out of D2 *)
+all: try solve [rewrite E2 in H; rewrite E2 in H1;
+  move: (C2 _ _ H H1) => h; inversion h].
+all: try solve [rewrite E1 in H; rewrite E1 in H2;
+  move: (C1 _ _ H H2) => h; inversion h].
+all: try solve [rewrite E2 in H0; rewrite E2 in H2;
+  move: (C2 _ _ H0 H2) => h; inversion h]. admit. 
++ (* both beta *)
+rewrite E1 in H; rewrite E1 in H2;
+move: (C1 _ _ H H2) => h.
+inversion h; subst. auto.
+rewrite E2 in H0. rewrite E2 in H3.
+move: H6 => [x1 [x2 [G1 [G2 I3]]]].
+have I4: List.In x1 F2. eapply H0. eauto. 
+have I5: List.In x2 F2. eapply H3. eauto.
+specialize (C2 _ _ I4 I5).
+assert False. eapply (disjoint_Consistent x1 x2); eauto. done.
++ (* both nth *)
+  rewrite E1 in H. rewrite E1 in H2.
+  rewrite E2 in H0. rewrite E2 in H3.
+  move: (C1 _ _ H H2) => h. inversion h. subst. clear h.
+  move: (C2 _ _ H0 H3) => h. inversion h. subst. clear h.
+  clear H0 H3 H H2.
+  move: k0 H1 H4.
+  induction H7. 
+  intros k0 hk; destruct k0; simpl in hk; try done.
+  intros k0 n1 n2; destruct k0; simpl in n1, n2.
+  inversion n1. inversion n2. subst. auto.
+  eapply IHForall2; eauto.
+Admitted.  
+
+specialize (C1 F1 E1).
+specialize (C2 F2 E2).
+unfold ConsistentAnyList in *.
+intros x y I1 I2.
+move: (h2 _ I1) => h1'.
+move: (h2 _ I2) => h2'.
+inversion h1'; subst; inversion h2'; subst; eauto.
+all: try solve [rewrite E1 in H; rewrite E1 in H0;
+  move: (C1 _ _ H H0) => h; inversion h].
+rewrite E2 in H. rewrite E2 in H1. admit. (* need to keep v_wrong out of D2 *)
+all: try solve [rewrite E2 in H; rewrite E2 in H1;
+  move: (C2 _ _ H H1) => h; inversion h].
+all: try solve [rewrite E1 in H; rewrite E1 in H2;
+  move: (C1 _ _ H H2) => h; inversion h].
+all: try solve [rewrite E2 in H0; rewrite E2 in H2;
+  move: (C2 _ _ H0 H2) => h; inversion h]. admit. 
++ (* both beta *)
+rewrite E1 in H; rewrite E1 in H2;
+move: (C1 _ _ H H2) => h.
+inversion h; subst. auto.
+rewrite E2 in H0. rewrite E2 in H3.
+move: H6 => [x1 [x2 [G1 [G2 I3]]]].
+have I4: List.In x1 F2. eapply H0. eauto. 
+have I5: List.In x2 F2. eapply H3. eauto.
+specialize (C2 _ _ I4 I5).
+assert False. eapply (disjoint_Consistent x1 x2); eauto. done.
++ (* both nth *)
+  rewrite E1 in H. rewrite E1 in H2.
+  rewrite E2 in H0. rewrite E2 in H3.
+  move: (C1 _ _ H H2) => h. inversion h. subst. clear h.
+  move: (C2 _ _ H0 H3) => h. inversion h. subst. clear h.
+  clear H0 H3 H H2.
+  move: k0 H1 H4.
+  induction H7. 
+  intros k0 hk; destruct k0; simpl in hk; try done.
+  intros k0 n1 n2; destruct k0; simpl in n1, n2.
+  inversion n1. inversion n2. subst. auto.
+  eapply IHForall2; eauto.
+Admitted.  
+*)
 
 (* ----------------------------------------------------- *)
 
@@ -599,6 +1182,41 @@ Proof.
 Qed.
 
 
+Lemma CONS_continuous {D E ρ}{w} :
+  (valid_env ρ)
+  -> w ∈ (CONS (D ρ) (E ρ))
+  -> continuous_env D ρ 
+  -> continuous_env E ρ
+  -> monotone_env D 
+  -> monotone_env E
+  -> exists ρ3 , 
+    exists (pf : finite_env ρ3) , ρ3 ⊆e  ρ 
+                             /\ (w ∈ (CONS (D ρ3) (E ρ3))).
+Proof.  
+  intros NE C. unfold CONS, In in C. destruct w.
+  all: try done.
+  destruct l. try done.
+  move: C => [Dv El].
+  intros IHD IHE mD mE.
+  destruct (IHD v Dv) as 
+      [ ρ1 [ fρ1 [ ρ1ρ VwDp1 ]]].
+  destruct (IHE (v_list l) El) as 
+      [ ρ2 [ fρ2 [ ρ2ρ VwDp2 ]]].
+  have S1: same_scope ρ1 ρ. eapply all2_same_scope; eauto.
+  have S2: same_scope ρ2 ρ. eapply all2_same_scope; eauto.
+  have SS: same_scope ρ1 ρ2. { transitivity ρ; auto. symmetry; auto. }
+  exists (ρ1 ⊔e ρ2).
+    repeat split.
+  - eapply join_finite_env; eauto.
+  - eapply join_lub; eauto.
+  - eapply mD. instantiate (1:= ρ1). 
+    eapply join_sub_left; eauto. auto.
+  - eapply mE. instantiate (1:= ρ2).
+    eapply join_sub_right; eauto. auto.
+Qed.
+
+
+
 Lemma APPLY_continuous {D E ρ}{w} :
   (valid_env ρ)
   -> w ∈ ((D ρ) ▩ (E ρ))
@@ -676,7 +1294,7 @@ Qed.
 
 Lemma Lambda_continuous {E ρ} {NE : valid_env ρ}{ v x} :
   v ∈ Λ (fun D => E (x ~ D ++ ρ)) 
-  -> (forall V, V <> nil -> not (v_wrong ∈ mem V) ->
+  -> (forall V, valid_mem V ->
           continuous_env E (x ~ mem V ++ ρ))
   -> monotone_env E
   -> exists ρ', exists (pf:finite_env ρ'),
@@ -686,8 +1304,8 @@ Proof.
   induction v.
   all: try solve [intros; cbv in H; done].
   - (* v is l ↦ v *)
-    intros [ wEVρ [VN NW] ] IH mE.
-    destruct (IH l VN NW v wEVρ) as
+    intros [ wEVρ NW ] IH mE.
+    destruct (IH l NW v wEVρ) as
       [ ρ' [ fρ' [ ρ'Vρ wEρ' ]]]. 
     inversion ρ'Vρ. subst. clear ρ'Vρ.
     inversion fρ'. subst. clear fρ'.
@@ -700,6 +1318,7 @@ Proof.
     repeat split; eauto.
 Qed.
 
+(*
 
 (* Exists *)
 
@@ -763,7 +1382,7 @@ Proof.
   auto.
 Qed.
 
-
+*)
 
 
 (* ---------------------------------------------------------- *)
@@ -799,7 +1418,6 @@ Proof.
   done.
 Qed.
 
-
 Lemma tm_induction : forall (P : tm -> Prop), 
     (forall i, P (var_b i)) 
     -> (forall x, P (var_f x)) 
@@ -807,20 +1425,25 @@ Lemma tm_induction : forall (P : tm -> Prop),
     -> (forall t, 
           (forall x , x `notin` fv_tm t -> P (t ^ x)) 
           -> P (abs t))
+    -> (forall k, P (lit k))
+    -> P add
+    -> P tnil
+    -> (forall t1 t2, P t1 -> P t2 -> P (tcons t1 t2))
     -> forall t, P t.
 Proof.
-  intros P VARB VARF APP ABS t.
+  intros P VARB VARF APP ABS LIT ADD NIL CONS t.
   remember (size_tm t) as n.
   have GE: n >= size_tm t. subst. auto. clear Heqn.
   move: t GE.
   induction (lt_wf n) as [n _ IH].
-  intros [ i | x | u | t ] SZ; simpl in SZ; eauto.
+  intros [ i | x | u | t | k | (* add *) | (* nil *) | t ] SZ; simpl in SZ; eauto.
   + eapply ABS.
     intros x FV.
     eapply (IH (size_tm u)). lia.
     autorewrite with lngen.
     lia.
-  + eapply APP; eapply IH; eauto. lia. lia.
+  + eapply APP; eapply IH; eauto; lia. 
+  + eapply CONS; eapply IH; eauto; lia. 
 Qed.    
 
 (* Denotation function: unbound variables have no denotation. *)
@@ -836,6 +1459,10 @@ Fixpoint denot_n (n : nat) (a : tm) (ρ : Env) : P Value :=
      | abs t => 
          let x := fresh_for (dom ρ \u fv_tm t) in 
          Λ (fun D => denot_n m (t ^ x) (x ~ D ++ ρ))
+     | lit k => NAT k
+     | add => ADD
+     | tnil => NIL
+     | tcons t u => CONS (denot_n m t ρ) (denot_n m u ρ)
      end
   end.
 
@@ -847,19 +1474,14 @@ Proof.
   induction (lt_wf n) as [n _ IH].
   intros a h ρ; destruct a; simpl in *.
   all: try destruct n; simpl; auto; try lia.
-  - f_equal.
-    extensionality D.
+  all: f_equal.
+  all: try rewrite IH; try lia; auto;
+    try rewrite IH; try lia; auto.
+  - extensionality D.
     remember (fresh_for (dom ρ \u fv_tm a)) as x.
     rewrite IH. lia.
     autorewrite with lngen. lia.
     autorewrite with lngen. auto.
-  - f_equal.
-    rewrite IH. lia. lia.
-    rewrite IH. lia. lia.
-    auto.
-    rewrite IH. lia. lia.
-    rewrite IH. lia. lia.
-    auto.
 Qed.
 
 Definition denot (a : tm) := denot_n (size_tm a) a.
@@ -883,6 +1505,25 @@ Proof.
   rewrite size_is_enough. lia. auto.
   rewrite size_is_enough. lia. auto.
 Qed.
+
+Lemma denot_lit : forall k ρ,  denot (lit k) ρ = NAT k.
+Proof. intros. reflexivity. Qed. 
+
+Lemma denot_add : forall ρ,  denot add ρ = ADD.
+Proof. intros. reflexivity. Qed. 
+
+Lemma denot_tnil : forall ρ,  denot tnil ρ = NIL.
+Proof.  intros. reflexivity. Qed. 
+
+Lemma denot_tcons : forall t u ρ, 
+    denot (tcons t u) ρ = CONS (denot t ρ) (denot u ρ).
+Proof. 
+  intros.
+  unfold denot. simpl.
+  rewrite size_is_enough. lia. auto.
+  rewrite size_is_enough. lia. auto.
+Qed.
+
 
 (* To compute the denotation of an abstraction, we need to first prove a
    renaming lemma. This lemma ensures that the names that we pick for the
@@ -980,6 +1621,10 @@ Proof.
     f_equal.
     apply IHn; simpl_env; auto.
     apply IHn; simpl_env; auto.
+  + simpl_env.
+    f_equal.
+    apply IHn; simpl_env; auto.
+    apply IHn; simpl_env; auto. 
 Qed.
 
 
@@ -1017,6 +1662,11 @@ Proof.
 Qed.
 
 
+Create HintDb denot.
+#[export] Hint Opaque denot : denot.
+#[export] Hint Rewrite denot_var_b denot_var denot_app denot_lit 
+  denot_add denot_tnil denot_tcons : denot.
+(* no hint for abs, must pick fresh first *)
 
 Lemma weaken_denot1 : forall t ρ ρ1 ρ2, 
     fv_tm t [<=] dom (ρ1 ++ ρ2) ->
@@ -1029,11 +1679,12 @@ Proof.
   2: move=>x.
   3: move=>t1 t2 IH1 IH2. 
   4: move=> u IH.
+  8: move=> t1 t2 IH1 IH2.
   all: intros ρ ρ1 ρ2 FV U.
   all: simpl_env in FV; simpl in FV. 
-  + repeat rewrite denot_var_b.
-    reflexivity.
-  + repeat rewrite denot_var.
+  all: autorewrite with denot.
+  all: try solve [reflexivity].
+  + (* var *) 
     destruct_uniq.
     move: (access_app_P ρ1 x) => [A1|A2].
     rewrite A1. rewrite A1. auto.
@@ -1044,7 +1695,7 @@ Proof.
     rewrite access_app_fresh; auto.
     intro h.
     solve_uniq.
-  + repeat rewrite denot_app.    
+  + (* app *)
     f_equal.
     eapply IH1; simpl_env; eauto.
     fsetdec.
@@ -1059,6 +1710,11 @@ Proof.
     rewrite <- app_assoc.
     erewrite IH; simpl_env; eauto.
     rewrite fv_tm_open_tm_wrt_tm_upper; simpl; eauto.
+    fsetdec.
+  + f_equal.
+    eapply IH1; simpl_env; eauto.
+    fsetdec.
+    eapply IH2; simpl_env; eauto.
     fsetdec.
 Qed.
 
@@ -1108,6 +1764,35 @@ Proof.
   fsetdec.
 Qed.
 
+
+Lemma scoped_tcons : forall t1 t2 ρ,
+    scoped t1 ρ -> scoped t2 ρ -> 
+    scoped (tcons t1 t2) ρ.
+Proof.
+  intros. inversion H. inversion H0. econstructor; eauto.
+  simpl. fsetdec.
+Qed.
+
+Lemma scoped_tcons_inv1 : forall t1 t2 ρ,
+    scoped (tcons t1 t2) ρ ->
+    scoped t1 ρ.
+Proof.
+  intros. inversion H.
+  simpl in *. inversion H2.
+  econstructor; eauto. 
+  fsetdec.
+Qed.
+
+Lemma scoped_tcons_inv2 : forall t1 t2 ρ,
+    scoped (tcons t1 t2) ρ ->
+    scoped t2 ρ.
+Proof.
+  intros. inversion H.
+  simpl in *. inversion H2.
+  econstructor; eauto. 
+  fsetdec.
+Qed.
+
 Lemma scoped_abs : forall x t1 D ρ, 
   x `notin` dom ρ \u fv_tm t1
   -> scoped (t1 ^ x) (x ~ D ++ ρ)
@@ -1145,9 +1830,12 @@ Lemma subst_denot : forall t x u ρ1 ρ2,
 Proof.
   intro t.
   eapply tm_induction with (t := t);
-  [move=>i|move=>y|move=>t1 t2 IH1 IH2|move=> t' IH].
+  [move=>i|move=>y|move=>t1 t2 IH1 IH2|move=> t' IH|move=>k| | | move=> t1 t2 IH1 IH2].
   all: intros x u ρ1 ρ2 ST SU.
-  + simpl. repeat rewrite denot_var_b. reflexivity.
+  all: simpl. 
+  all: simpl_env. 
+  all: autorewrite with denot.
+  all: try solve [reflexivity].
   + destruct (y == x) eqn:EQ. subst.
     ++ have NI: x `notin` dom ρ1.
        { inversion ST. destruct_uniq. auto. }
@@ -1155,13 +1843,10 @@ Proof.
        { inversion SU. auto. }
        have U2: uniq (ρ1 ++ ρ2). 
        { inversion ST. solve_uniq. }
-       rewrite subst_eq_var.
-       rewrite denot_var.
        rewrite access_app_fresh; auto.       
        rewrite access_eq_var.
        apply weaken_denot; eauto.
-    ++ rewrite subst_neq_var; auto.
-       repeat rewrite denot_var.
+    ++ repeat rewrite denot_var.
        destruct (access_app_P ρ1 y) as [h1 | h2].
        repeat rewrite h1. auto.
        move: (h2 ρ2) => [N1 ->]. 
@@ -1169,7 +1854,6 @@ Proof.
        rewrite access_neq_var; auto.
   + move: (scoped_app_inv1 _ _ _ ST) => S1.
     move: (scoped_app_inv2 _ _ _ ST) => S2.
-    simpl. repeat rewrite denot_app.
     f_equal.
     eapply IH1; eauto.
     eapply IH2; eauto.
@@ -1190,6 +1874,11 @@ Proof.
     autorewrite with lngen.
     reflexivity.
     auto.
+  + move: (scoped_tcons_inv1 _ _ _ ST) => S1.
+    move: (scoped_tcons_inv2 _ _ _ ST) => S2.
+    f_equal.
+    eapply IH1; eauto.
+    eapply IH2; eauto.
 Qed.
 
 Lemma subst_denot1 :
@@ -1223,14 +1912,12 @@ Lemma denot_monotone {t}:
 Proof.
   unfold monotone_env.
   eapply tm_induction with (t := t);
-  [move=>i|move=>y|move=>t1 t2 IH1 IH2|move=> t' IH].
+  [move=>i|move=>y|move=>t1 t2 IH1 IH2|move=> t' IH|move=>k| | | move=> t1 t2 IH1 IH2].
  all: intros ρ ρ' S.
-  + repeat rewrite denot_var_b. 
-    reflexivity.
-  + repeat rewrite denot_var.
-    eapply access_monotone; auto.
-  + repeat rewrite denot_app.
-    eapply APPLY_mono_sub; eauto.
+ all: autorewrite with denot.
+ all: try solve [reflexivity].
+  + eapply access_monotone; auto.
+  + eapply APPLY_mono_sub; eauto.
   + pick fresh x.
     repeat rewrite (denot_abs x).
     fsetdec.
@@ -1239,6 +1926,7 @@ Proof.
     intros X NE.
     eapply IH. fsetdec.
     eapply extend_sub_env; eauto. 
+  + eapply CONS_mono_sub; eauto.
 Qed.
 
 
@@ -1254,20 +1942,26 @@ Proof.
   econstructor; eauto.
 Qed.
   
+Lemma valid_nonempty_mem : forall V, 
+      valid_mem V -> nonemptyT (mem V).
+Proof. intros.
+       destruct V. inversion H. 
+       unfold nonemptyT. exists v. eauto.
+Qed.
+
 (* ⟦⟧-continuous *)
 Lemma denot_continuous {t} : forall ρ,
     valid_env ρ
   -> continuous_env (denot t) ρ.
 Proof.
   eapply tm_induction with (t := t);
-  [move=>i|move=>x|move=>t1 t2 IH1 IH2|move=> t' IH].
+  [move=>i|move=>x|move=>t1 t2 IH1 IH2|move=> t' IH|move=>k| | | move=> t1 t2 IH1 IH2].
   all: intros ρ NE.
   all: intros v vIn.
-  + rewrite denot_var_b in vIn. 
-    exists (initial_finite_env ρ NE).
-    eexists; eauto.
-  + rewrite denot_var in vIn.
-    destruct (FSetDecideAuxiliary.dec_In x (dom ρ)).
+  all: autorewrite with denot in vIn.
+  all: try solve [ exists (initial_finite_env ρ NE);
+    eexists; eauto] .
+  + destruct (FSetDecideAuxiliary.dec_In x (dom ρ)).
     - exists (single_env x ⌈ v ⌉ ρ NE).
       exists (@single_fin v x ρ NE).
       split.
@@ -1278,8 +1972,7 @@ Proof.
       rewrite denot_var.
       rewrite access_fresh. simpl_env. auto.
       rewrite access_fresh in vIn. auto. done.
-  + rewrite denot_app in vIn.
-    edestruct (APPLY_continuous NE vIn) as [ρ' [F SS]]; eauto.
+  + edestruct (APPLY_continuous NE vIn) as [ρ' [F SS]]; eauto.
     eapply denot_monotone.
     eapply denot_monotone.
     exists ρ'. exists F.
@@ -1289,15 +1982,18 @@ Proof.
     move: (@Lambda_continuous _ _ NE v x vIn) => h.    
     destruct h as [ρ' [Fρ' [S vvIn]]].
     ++ intros V NEV NW.
-       move: (nonnil_nonempty_mem NEV) => [w h0]. 
+       move: (valid_nonempty_mem _ NEV) => [w h0]. 
        eapply IH; eauto.
-       eapply extend_valid_env; eauto.
-       econstructor; eauto.
     ++ eapply denot_monotone.
     ++ exists ρ'. exists Fρ'. 
        erewrite <- all2_dom in Fr. 2: eapply S.
        rewrite (denot_abs x). fsetdec.
        split; auto.
+  + edestruct (CONS_continuous NE vIn) as [ρ' [F SS]]; eauto.
+    eapply denot_monotone.
+    eapply denot_monotone.
+    exists ρ'. exists F.
+    rewrite denot_tcons. auto.
 Qed.
 
 
@@ -1315,6 +2011,7 @@ Proof.
   eapply denot_continuous; auto.
 Qed.
 
+
 Definition Same_env : Env -> Env -> Prop := all2 Same_set.
 
 (* The denotation respects ≃ *)
@@ -1322,17 +2019,16 @@ Instance Proper_denot : Proper (eq ==> Same_env ==> Same_set) denot.
 Proof.
   intros t1 t ->.
   eapply tm_induction with (t := t);
-  [move=>i|move=>x|move=>t1 t2 IH1 IH2|move=> t' IH].
+  [move=>i|move=>x|move=>t1 t2 IH1 IH2|move=> t' IH|move=>k| | | move=> t1 t2 IH1 IH2].
   all: move => ρ1 ρ2 EQ.
-  - repeat rewrite denot_var_b. reflexivity.
-  - repeat rewrite denot_var.
-    destruct (FSetDecideAuxiliary.dec_In  x (dom ρ1)).
+  all: autorewrite with denot.
+  all: try solve [reflexivity].
+  all: eauto using APPLY_cong, CONS_cong.
+  - destruct (FSetDecideAuxiliary.dec_In  x (dom ρ1)).
     + apply all2_access with (f := Same_set); auto.
     + rewrite access_fresh. auto.
       rewrite access_fresh. erewrite all2_dom in H; eauto.
       reflexivity.
-  - repeat rewrite denot_app. 
-    eauto using APPLY_cong.
   - pick fresh x. 
     repeat rewrite (denot_abs x). fsetdec. fsetdec.
     eapply Λ_ext.
@@ -1347,17 +2043,16 @@ Instance Proper_sub_denot : Proper (eq ==> all2 Included ==> Included) denot.
 Proof.
   intros t1 t ->.
   eapply tm_induction with (t := t);
-  [move=>i|move=>x|move=>t1 t2 IH1 IH2|move=> t' IH].
+  [move=>i|move=>x|move=>t1 t2 IH1 IH2|move=> t' IH|move=>k| | | move=> t1 t2 IH1 IH2].
   all: move => ρ1 ρ2 SUB.
-  - repeat rewrite denot_var_b. reflexivity.
-  - repeat rewrite denot_var.
-    destruct (FSetDecideAuxiliary.dec_In  x (dom ρ1)).
+  all: autorewrite with denot.
+  all: try solve [reflexivity].
+  all: eauto using APPLY_mono_sub, CONS_mono_sub.
+  - destruct (FSetDecideAuxiliary.dec_In  x (dom ρ1)).
     + apply all2_access with (f := Included); auto.
     + rewrite access_fresh. auto.
       rewrite access_fresh. erewrite all2_dom in H; eauto.
       reflexivity.
-  - repeat rewrite denot_app.  
-    eauto using APPLY_mono_sub.
   - pick fresh x. 
     repeat rewrite(denot_abs x). fsetdec. fsetdec.
     eapply Λ_ext_sub.
@@ -1391,7 +2086,7 @@ Proof.
     rewrite <- S. reflexivity.
     rewrite <- SUB.
     auto.
-    auto.
+    eapply valid_sub_valid_mem; eauto. rewrite <- S. auto.
 Qed.
 
 (* Λ⟦⟧-▪-id *)
@@ -1417,7 +2112,7 @@ Qed.
 
 Definition tm_Id : tm := abs (var_b 0).
 
-Lemma denot_Id : ( v_fun :: nil ↦ v_fun) ∈ denot tm_Id nil.
+Lemma denot_Id : (v_fun :: nil ↦ v_fun) ∈ denot tm_Id nil.
 Proof.
   unfold tm_Id.
   pick fresh x.
@@ -1425,34 +2120,54 @@ Proof.
   cbv.
   destruct (KeySetFacts.eq_dec x x); try done.
   split. left. auto.
-  split. intro h. done. 
+  split. left. auto.  
   intros [v1| v2]; done.
 Qed. 
+
+
+Lemma denot_Id_inv : forall x ρ, x ∈ denot tm_Id ρ ->
+                          forall w, Consistent x (w :: nil ↦ w).
+Proof.
+  intros x ρ.
+  unfold tm_Id. 
+  pick fresh y.
+  rewrite (denot_abs y); auto.
+  intro h. unfold In in h. 
+  unfold Λ in h.
+  destruct x; try done.
+  move: h => [h0 h1].
+  cbn in h0. rewrite eq_dec_refl in h0.
+  unfold valid_mem in h1. destruct l. done.
+  unfold valid_witness in h1. destruct h1 as [_ h3].
+  unfold mem in h0, h3.
+  unfold In in h3.
+  intro w.
+Admitted.
+
 
 Definition tm_Delta : tm := abs (app (var_b 0) (var_b 0)).
 
 
 #[global] Hint Rewrite access_eq_var : lngen.
 
-Lemma denot_Delta_inv : forall (v : Value), 
-    v ∈ denot tm_Delta nil -> 
-    (exists v1 w, v = (((v1 :: nil ↦ w) :: v1 :: nil) ↦ w) /\ w <> v_wrong) \/ v = v_fun.
+Lemma denot_Delta_inv :
+  forall x, x ∈ denot tm_Delta nil -> 
+       exists v w, Consistent x (((v :: nil ↦ w) :: v :: nil) ↦ w).
 Proof.
-  intros v.
-  unfold tm_Delta.
-  pick fresh x.
-  rewrite (denot_abs x); auto.
-  unfold Λ.
-  autorewrite with lngen.
-  destruct v; intro h; try done.
-  unfold In in h.
-  rewrite denot_app in h. 
-  rewrite denot_var in h.
-  rewrite access_eq_var in h.
-  move: h => [D1 [ne nw]].
-  inversion D1; subst; try done.
-  destruct V; try done.  
-Abort.    
+  intro x.  unfold In, tm_Delta.
+  pick fresh y.
+  rewrite (denot_abs y); auto.
+  cbn. rewrite eq_dec_refl.
+  unfold Λ. destruct x; try done.
+  move=> [h0 h1].
+  inversion h0; subst. 
+  + unfold valid_mem, valid_witness in h1.
+    destruct l. done. destruct h1. done.
+  + unfold valid_mem, valid_witness in h1.  
+    destruct l. done. destruct h1. done.
+  + unfold In in H. unfold mem in H. 
+    admit.
+Admitted.
 
 Lemma denot_Delta : forall (v w : Value), v <> v_wrong ->
     (((v :: nil ↦ w) :: v :: nil) ↦ w) ∈ denot tm_Delta nil.
@@ -1469,9 +2184,10 @@ Proof.
   unfold In. left. auto.
   rewrite -> mem_singleton. 
   intros x0 II. inversion II. subst. cbv. right. left. auto.
-  intro h. done.
-  intro h. apply NW. inversion h. auto. inversion H.
-  split. intro h. done.
+  unfold valid_mem, valid_witness.
+  split; eauto.
+  intro h. inversion h. done. inversion H.
+  split. eauto. 
   intros [v1|[v2|v3]]; try done.
 Qed.
 
@@ -1520,7 +2236,9 @@ Proof.
     simpl in FV. fsetdec.
   + pick fresh x.
     erewrite denot_abs with (x:=x); eauto.
-Qed. 
+    eapply valid_Λ.
+  + 
+Admitted.
 
 Lemma soundness: 
   forall t u, 
@@ -1544,7 +2262,7 @@ Proof.
     fsetdec.
     auto.
     fsetdec.
-    rewrite (subst_tm_intro x t u); auto.
+    rewrite (subst_tm_intro x t v); auto.
     replace ρ with (nil ++ ρ) at 3.
     rewrite <- subst_denot with (ρ1 := nil). reflexivity.
     simpl_env.
@@ -1582,4 +2300,6 @@ Proof.
     repeat rewrite denot_app.
     eapply APPLY_cong; eauto.
     reflexivity.
-Qed.
+Admitted.
+
+
