coq/relations_full.v
@@ -1,0 +1,989 @@
+Require Export lc.tactics.
+Import LCNotations.
+Local Open Scope lc_scope.
+
+
+(*** Formalization of Barendregt's Chapter 3 (REDUCTION). *)
+
+
+(* ################################################################# *)
+(** * Section 3.1 Notions of reduction *)
+
+(** We start by defining *properties* of binary term relations.
+  
+    In our Ott generated definitions, a [relation] is defined as the type
+    [tm -> tm -> Prop]. 
+
+    Below, we'll use the metavariable [R] for relations, and if terms [t] and 
+    [u] are related by [R], then we will write that as [R t u].
+
+    Because we are working with a locally nameless representation, if we have 
+    [R t u], we'll want to know that both [t] and [u] are locally closed. In 
+    other words, we have satisfied the [lc R] constraint.
+
+ *)
+
+(** ** Equivalence relation (and type classes) *)
+
+(** This is a standard mathematical definitions. An *equivalence* relation is
+    one that is reflexive, symmetric and transitive.  These definitions are
+    similar to those in the the Coq standard library
+    (https://coq.inria.fr/library/Coq.Classes.RelationClasses.html) but note
+    that reflexivity is only required for *locally closed* terms.
+
+    A type class is a form of record type that is determined by its parameter
+    [R]. We expect that there will only be one meaningful way that a relation
+    can be reflexive. Later on, we will create values of this record type for
+    specific relations by supplying appropriate proofs. By declaring these
+    records asw type classes, Coq can find these proofs automatically, just by
+    knowing what relation we are working with.  *)
+
+Class reflexive (R: relation) := {
+  reflexivity : forall t : tm, lc_tm t -> R t t
+}.
+Class transitive (R: relation) := {
+  transitivity : forall t1 t2 t3 : tm, R t1 t2 -> R t2 t3 -> R t1 t3
+}.
+Class symmetric (R: relation) := {
+  symmetry : forall t1 t2 : tm, R t1 t2 -> R t2 t1
+}.
+
+Class equivalence (R : relation) : Prop := {
+    equivalence_reflexive  :> reflexive R ;
+    equivalence_symmetric  :> symmetric R ;
+    equivalence_transitive :> transitive R 
+}.
+
+(* ================================================================= *)
+
+(** ** Compatible relation *)
+
+(** Definition 3.1.1 (i)
+
+   A *compatible* relation is one that is preserved by the constructors of the
+   language definition. We might write this informally, using the three
+   conditions.
+
+       - (abs) R t u implies R \x.t \x.u
+
+       - (app1) R t t' implies R (t u) (t' u)
+
+       - (app2) R u u' implies R (t u) (t u')
+
+   Because of our use of the locally nameless representation, we'll need to 
+   add lc_tm preconditions to `compatible_app1` and `compatible_app2`.
+
+   Also, compatibility for the `abs` constructor is stated in the "exists-fresh"
+   form. We need to be able to show that the relation holds for a single 
+   variable that is sufficiently fresh.
+
+ *)
+
+
+
+Class compatible (R: relation) := {
+
+    compatible_abs :  forall x t u,
+      x `notin` fv_tm t \u fv_tm u ->
+      R (t ^ x)(u ^ x) -> R (abs t) (abs u) ;
+
+    compatible_app1 : forall t t' u, 
+      R t t' -> lc_tm u -> R (app t u) (app t' u) ;
+
+    compatible_app2 : forall t u u', 
+      lc_tm t -> R u u' -> R (app t u) (app t u') ;
+
+    compatible_cons1 : forall t t' u, 
+      R t t' -> lc_tm u -> R (tcons t u) (tcons t' u) ;
+
+    compatible_cons2 : forall t u u', 
+      lc_tm t -> R u u' -> R (tcons t u) (tcons t u')
+  }.
+
+(** In the case when the relation is reflexive and transitive, we can use the
+    two separate properties for application at once. The notation `{_} marks 
+    type class arguments to this lemma. When we apply the lemma, Coq will 
+    search for the values automatically. *)
+
+Lemma compatible_app {R} `{lc R} `{reflexive R} `{transitive R} `{compatible R} :
+  forall t u t' u',
+  R t t' -> R u u' -> R (app t u) (app t' u').
+Proof.
+  (* WORKED IN CLASS *)
+  intros. 
+  eapply transitivity with (t2 := (app t' u)).
+  eapply compatible_app1; eauto with lngen.  
+  eapply compatible_app2; eauto with lngen.
+Qed. 
+Lemma compatible_cons {R} `{lc R} `{reflexive R} `{transitive R} `{compatible R} :
+  forall t u t' u',
+  R t t' -> R u u' -> R (tcons t u) (tcons t' u').
+Proof.
+  (* WORKED IN CLASS *)
+  intros. 
+  eapply transitivity with (t2 := (tcons t' u)).
+  eapply compatible_cons1; eauto with lngen.  
+  eapply compatible_cons2; eauto with lngen.
+Qed. 
+
+(* ================================================================= *)
+
+(** Definition 3.1.1 (ii) a *congruence* relation (also called an equality) is 
+   a compatible equivalence relation. *)
+Class congruence R := {
+  congruence_equivalence :> equivalence R ;
+  congruence_compatible  :> compatible R 
+}.
+
+(** Definition 3.1.1 (iii) a *reduction* relation is reflexive, transitive and 
+  compatible. *)
+Class reduction R := {
+  reduction_reflexive  :> reflexive R ;
+  reduction_transitive :> transitive R ;
+  reduction_compatible :> compatible R
+}.
+
+
+(** We'll jump ahead a bit in the chapter and also define the following three
+    substitution properties for binary term relations.
+
+    In general, we expect the first property to always hold for any binary
+    term relation. If two terms are related, then they should still be 
+    related after substitution.
+
+    However, the second and third may or may not be true.  (For example, the
+    second is not true for primitive "beta" reduction.)  *)
+
+(** Definition 3.1.14 *)
+Definition subst1 (R : relation) := 
+  forall t t' x u, lc_tm u -> value u ->
+    R t t' -> R (t [ x ~> u ]) (t' [ x ~> u ]) .
+Definition subst2 (R : relation) :=
+  forall x t u u', lc_tm t -> value u ->
+    R u u' -> R (t [ x ~> u ]) (t [ x ~> u' ]).
+Definition subst3 (R : relation) :=
+  forall x t t' u u', 
+    value u -> value u' ->
+    R t t' -> R u u' -> R (t [ x ~> u ]) ( t' [ x ~> u' ]).
+
+(** We'll also make a class for relations that satisfy the first substitution
+    property. *)
+Class substitutive (R : relation) := {
+    subst : subst1 R
+}.
+
+(** Finally, we'll say that a relation S is a closure of relation R if it 
+    includes everything that is related by R (and possibly more things.
+ *)
+Class closure (R S : relation) := { 
+    embed : forall t u, R t u -> S t u
+  }.
+
+
+(* ================================================================= *)
+
+(** ** Definition 3.1.4 and 3.1.5
+    
+   Next, We will diverge slightly from Barendregt and use a general definition
+   for reflexive-transitive closure and symmetric-transitive closure instead
+   of layering them on top of compatible closure.
+
+   Take a moment to look at the following inductive definitions that appear in
+   the Ott file. These definitions are a way of taking a relation and forcing
+   it to be compatible, reflexive, and transitive.  *)
+
+Print compatible_closure.
+Print refl_trans_closure.
+Print sym_trans_closure.
+ 
+(** Below are some names for specific closures of R. Below, we will call an
+    arbitrary [R] a "reduction" and imagine it as a step or transition
+    rule. i.e. if we have [R t u] then we say "[t] reduces to [u] via [R]".  *)
+
+(** Allow exactly one R-reduction, anywhere inside the term. *)
+Definition one_step_R_reduction (R : relation) := compatible_closure R.
+
+(** Allow a sequence of arbitrarily many one step R-reductions *)
+Definition R_reduction (R : relation) := refl_trans_closure (compatible_closure R).
+
+(** Generate congruence relation from R-reduction, by forcing it 
+    to also be symmetric. *)
+Definition R_convertibility (R : relation) := sym_trans_closure (R_reduction R).
+
+(** We will also specialize the latter definitions to the [beta] relation *)
+
+Definition beta_reduction := R_reduction beta.
+Definition beta_convertibility := R_convertibility beta.
+
+(** Note: beta_convertibility is almost the same as beta_equivalence. However,
+    beta_equivalence is defined directly as the reflexive, symmtric,
+    transitive, compatible closure of beta_reduction, which is not quite the
+    same as the above proof. Both definitions do relate the same terms, but
+    beta_equivalence derivations are less structured than beta_conversion.
+
+    If each of the \ and / below are beta_reductions, then a
+    beta_convertibility proof looks like:
+
+            t t1 t2 ...  t3 u \ / \ / \ / \ / t' t1' ...  u' *)
+
+
+(* ================================================================= *)
+
+Lemma lc_value : forall v, value v -> lc_tm v.
+Proof.
+  induction 1; eauto.
+Qed.
+
+#[export] Hint Resolve lc_value : core.
+
+Lemma lc_nth : forall v k w, lc_tm v -> nth v k = Some w -> lc_tm w.
+Proof.
+  move=>v k w V. move: k w.
+  induction V; simpl; intro h; try done; eauto.
+  move=> w h0; destruct h; try done.
+  inversion h0. subst. eauto. eauto.
+Qed.
+
+#[export] Hint Immediate lc_nth : core.
+
+Lemma value_nth : forall v k w, value v -> nth v k = Some w -> value w.
+Proof.
+  move=>v k w V. move: k w.
+  induction V; simpl; intro h; try done; eauto.
+  move=> w0 h0; destruct h; try done.
+  inversion h0. subst. eauto. eauto.
+Qed.
+
+#[export] Hint Immediate value_nth : core.
+
+
+Lemma subst_nth : forall v k w x u, nth v k = Some w ->  nth (v [x ~> u]) k = Some (w [x ~> u]).
+Proof.
+  induction v; simpl; intros; try done.
+  destruct k. inversion H. subst. auto. 
+  eauto.
+Qed.
+
+#[export] Hint Immediate subst_nth : core.
+
+(** We'll want to show that beta_reduction and beta_convertibility have the
+    properties listed above. We can do so by proving those properties about
+    the closure operations and asking Coq to glue these results together 
+    via type class resolution. 
+
+ *)
+
+Lemma  is_value_subst : forall v x u, is_value v -> is_value u -> is_value (v [x ~> u]).
+Proof. induction v; intros; simpl; eauto. 
+       destruct (x == x0); eauto.
+       inversion H.
+       split; eauto.
+Qed.
+
+#[export] Hint Resolve is_value_subst : core.
+
+
+Lemma  value_subst : forall v x u, value v -> value u -> value (v [x ~> u]).
+Proof. induction v; intros; simpl; eauto with lngen. 
+       destruct (x == x0); eauto.
+       admit.
+       inversion H.
+       inversion H; eauto.
+Admitted.
+
+#[export] Hint Resolve value_subst : core.
+
+
+(** ** Properties of the compatible closure operation *)
+
+#[local]
+Instance lc_compatible_closure {R} `{lc R} : lc (compatible_closure R).
+Proof.
+  split.
+  - intros a b CC. induction CC; eauto using lc1.
+  - intros a b CC. induction CC; eauto using lc2.
+Qed. 
+
+#[local]
+Instance closure_compatible_closure {R} : closure R (compatible_closure R).
+Proof. constructor. intros; eauto using cc_rel. Qed.
+
+(** *** Exercise [subst1_compatible closure] *)
+
+(** This is a standard substitution lemma *)
+#[local]
+Instance subst1_compatible_closure R { SR : substitutive R } : substitutive (compatible_closure R).
+Proof. 
+(* FILL IN HERE *) Admitted.
+
+(** Due to the use of co-finite quantification in our definition of
+    compatible_closure (in the Ott file), we need the underlying relation to
+    be substitutive.  Showing this result is similiar to proving an
+    "exists-fresh" lemma *)
+
+#[local]
+Instance compatible_compatible_closure {R} `{substitutive R} : compatible (compatible_closure R).
+Proof.
+    (* WORKED IN CLASS *)
+  split;  intros; eauto.
+  have SS: substitutive (compatible_closure R) by typeclasses eauto.
+  pick fresh y and apply cc_abs.
+  rewrite (subst_tm_intro x t); auto.
+  rewrite (subst_tm_intro x u); auto.
+  eapply subst; eauto.
+Admitted.
+
+(** ** Properties of refl_trans_closure operation **)
+
+(** *** Exercise [lc_refl_trans_closure] *)
+
+#[local]
+Instance lc_refl_trans_closure {R} `{lc R} : lc (refl_trans_closure R).
+Proof. (* FILL IN HERE *) Admitted.
+
+#[local]
+Instance closure_refl_trans_closure {R} : closure R (refl_trans_closure R).
+Proof. constructor. intros; eauto using rt_rel. Qed.
+
+#[local]
+Instance reflexive_refl_trans_closure {R}: reflexive (refl_trans_closure R).
+Proof. constructor. intros. eauto using rt_refl with lngen. Qed.
+
+#[local]
+Instance transitive_refl_trans_closure {R} : transitive (refl_trans_closure R).
+Proof. constructor. intros. eauto using rt_trans with lngen. Qed.
+
+#[local]
+Instance subst1_refl_trans_closure {R} `{substitutive R} : substitutive (refl_trans_closure R).
+Proof.
+  constructor. unfold subst1.
+  intros t t' x u LC Vu RTC.
+  induction RTC; eauto using subst with lngen.
+Qed.
+
+#[local]
+Instance compatible_refl_trans_closure {R} `{compatible R} : 
+  compatible (refl_trans_closure R).
+Proof.
+  (* WORKED IN CLASS *)
+  split;  intros x t u H1 H0; eauto.
+  + dependent induction H0. 
+    - (* rt_rel *)
+      eapply rt_rel. 
+      eapply (compatible_abs x); eauto.
+    - (* rt_refl *)
+      autorewrite with lngen in x. subst. 
+      eapply reflexivity; eauto with lngen.
+    - (* rt_trans *) 
+      eapply transitivity with (t2 := abs (close x t2)).
+      eapply IHrefl_trans_closure1 with (x := x); auto;
+      autorewrite with lngen; auto.
+      eapply IHrefl_trans_closure2 with (x:= x); auto;
+      autorewrite with lngen; auto.
+  + dependent induction H1; eauto using compatible_app1.
+  + dependent induction H0; eauto using compatible_app2.
+  + dependent induction H1; eauto using compatible_cons1.
+  + dependent induction H0; eauto using compatible_cons2.
+Qed. 
+
+(** ** Properties of sym_trans_closure: it preserves local closure,
+substitutivity and compatibility *)
+
+(** *** Exercise [lc_sym_trans_closure] *)
+#[local]
+Instance lc_sym_trans_closure {R} `{lc R} : lc (sym_trans_closure R).
+Proof.  (* FILL IN HERE *) Admitted.
+
+#[local]
+Instance closure_sym_trans_closure {R} : closure R (sym_trans_closure R).
+Proof. constructor. intros; eauto using st_rel. Qed.
+
+#[local]
+Instance symmetric_sym_trans_closure {R} : symmetric (sym_trans_closure R).
+Proof. constructor. intros. eauto using st_sym with lngen. Qed.
+
+#[local]
+Instance transitive_sym_trans_closure {R} : transitive (sym_trans_closure R).
+Proof. constructor. intros. eauto using st_trans with lngen. Qed.
+
+#[local]
+Instance reflexive_sym_trans_closure {R} `{reflexive R} : 
+  reflexive (sym_trans_closure R).
+Proof. constructor. intros. apply embed. apply reflexivity. auto. Qed.
+
+#[local]
+Instance subst1_sym_trans_closure {R} {SR : substitutive R} : substitutive (sym_trans_closure R).
+Proof.
+  constructor. unfold subst1. intros t t' x u LCu Vu STC.
+  induction STC.
+  - eapply embed; eauto using subst. 
+  - eapply symmetry; eauto.
+  - eapply transitivity with (t2 := t2 [x ~> u]); eauto.
+Qed.
+
+(** *** Exercise [compatible_sym_trans_closure] *)
+
+#[local]
+Instance compatible_sym_trans_closure {R} {CR: compatible R} : compatible (sym_trans_closure R).
+Proof.
+  (* FILL IN HERE *) Admitted.
+
+(* ================================================================= *)
+
+(** Now let's put everything together and show properties of R-reduction and R-convertibility. *)
+
+(** ** Lemma 3.1.6  
+
+   Our definition of the R_reduction operation produces a reduction relation
+   and R_convertibility produces a congruence relation. 
+   
+*)
+
+#[local]
+Instance reduction_R_reduction R `{substitutive R} : reduction (R_reduction R).
+Proof.
+  split; typeclasses eauto.
+Qed.
+
+#[local]
+Instance congruence_R_convertibility {R} `{substitutive R}: congruence (R_convertibility R).
+Proof.
+  split.
+  - split; typeclasses eauto.
+  - typeclasses eauto. 
+Qed.
+
+
+(** ** Remark 3.1.7 *)
+
+Lemma subst2_R_reduction R `{lc R}`{substitutive R}: subst2 (R_reduction R).
+Proof.
+  (* WORKED IN CLASS *)
+  unfold subst2. 
+  intros x t u u' LCt Vu Red.
+  have LC: lc (refl_trans_closure (compatible_closure R)). { typeclasses eauto. }
+  have CC: compatible (refl_trans_closure (compatible_closure R)). { typeclasses eauto. }
+  (* induction on the "syntax" of the term *)
+  induction LCt; simpl; eauto.
+  all: try eapply reflexivity; eauto.
+  + (* var *)
+    destruct_var_eq.
+    auto.
+    eapply reflexivity; auto.
+  + (* abs *) 
+    pick fresh y. spec y.
+    eapply compatible_abs with (x:=y).
+    autorewrite with lngen. auto.
+    rewrite_subst_open_hyp; eauto with lngen.    
+  + (* app *)
+    eapply compatible_app; eauto.
+  + (* list *) 
+    eapply compatible_cons; eauto.
+Qed.
+
+(* ================================================================= *)
+
+(** The next part defines what it means for a term to be a normal
+    form [nf] according to some reduction relation R. 
+  *)
+
+(** ** Definition 3.1.8 *)
+
+(** (i) A term t is a R-redex if there exists u, such that R t u *)
+Print redex.
+
+(** (ii) A term t is R-normal-form if no subterm contains an R-redex *)
+Print nf.
+
+(** (iii) A term u is a R-nf-of t if u is an R-nf and t is R-convertible to u. *)
+Definition R_nf_of R u t := nf R u /\ R_convertibility R t u.
+
+(** ** Lemma 3.1.10  (i) *)
+
+(** Normal forms do not single-step *)
+
+Lemma nf_normal R : forall t,
+  nf R t -> not (redex (compatible_closure R) t).
+Proof.
+  intros t nft.
+  induction nft.
+  all: intros h; inversion h; subst.
+  all: match goal with [H0 : compatible_closure ?R ?x ?u |- _ ] => inversion H0; subst end; eauto. 
+  pick fresh x. spec x. eauto.
+Qed.
+
+(** ** Lemma 3.1.10  (ii) *)
+
+(** Normal forms only reduce to themselves *)
+
+Lemma nf_noreduction {R} : forall t,  nf R t -> forall u, R_reduction R t u -> t = u /\ nf R u.
+Proof.
+  intros.
+  unfold R_reduction in H0. 
+  dependent induction H0.
+  - apply nf_normal in H.
+    apply False_ind. apply H.
+    exists u. auto.
+  - auto.
+  - destruct (IHrefl_trans_closure1 R); auto. subst.
+    destruct (IHrefl_trans_closure2 R); auto.
+Qed.
+
+(* ================================================================= *)
+
+(** ** Definition 3.1.11 *) 
+
+Definition diamond_property (R : relation) := 
+  forall t t1 t2, R t t1 -> R t t2 -> exists t3, R t1 t3 /\ R t2 t3.
+
+Definition church_rosser (R : relation) := diamond_property (R_reduction R).  
+
+(** ** Theorem 3.1.12 *)
+
+(** R-compatible terms R-reduce to a common term *)
+
+Theorem convertibility_reduction_diamond {R} `{lc R} (CR: church_rosser R) :
+  forall t u, R_convertibility R t u -> exists z, R_reduction R t z /\ R_reduction R u z.
+Proof. 
+  intros t u Rconv.
+  have lcRR: lc (R_reduction R). { typeclasses eauto. }
+  unfold R_convertibility in *.
+  dependent induction Rconv.
+  - exists u. split; unfold R_reduction. auto. eapply reflexivity. eapply lc2; eauto.
+  - edestruct (IHRconv R) as [z [Ruz Rtz]]; eauto.
+  - edestruct (IHRconv1 R) as [z1 [Rt1z1 Rt2z1]]; eauto.
+    edestruct (IHRconv2 R) as [z2 [Rt2z2 Rt3z2]]; eauto.
+    unfold church_rosser, diamond_property in CR.
+    destruct (CR _ _ _ Rt2z1 Rt2z2) as [z3 [Rz1z3 Rz2z3]]; eauto.
+    (*      t1     t2    t3
+               z1     z2
+                   z3           *)
+    exists z3. split. 
+    eapply transitivity with (t2:= z1); eauto.
+    eapply transitivity with (t2:= z2); eauto.
+Qed.
+
+
+(** ** Corollary 3.1.13 *)
+Lemma nf_reduce R `{lc R} (CR: church_rosser R) : forall u t, R_nf_of R u t -> R_reduction R t u.
+Proof.
+  intros u t.
+  unfold R_nf_of.
+  intros [NF RC].
+  destruct (convertibility_reduction_diamond CR _ _ RC) as [z[Rtz Rzu]].
+  edestruct (nf_noreduction _ NF _ Rzu). subst.
+  auto.
+Qed.
+  
+(** ** Proposition 3.1.15 *)
+
+#[local]
+Instance subst1_R_reduction {R} `{substitutive R} : substitutive (R_reduction R).
+Proof.
+  typeclasses eauto.
+Qed.
+
+#[local]
+Lemma subst1_R_convertibility {R} `{substitutive R} : substitutive (R_convertibility R).
+Proof.
+  typeclasses eauto.
+Qed.
+
+(** ** Proposition 3.1.16 *)
+
+(** *** Exercise [subst1_beta] *)
+
+#[local]
+Instance subst1_beta : substitutive beta.
+Proof. (* FILL IN HERE *) Admitted.
+
+(* ================================================================= *)
+
+(** ** Definition 3.2.3 is often called parallel reduction. *)
+
+Print parallel.
+
+(** Properties of parallel reduction *)
+
+#[local]
+Instance lc_parallel : lc parallel.
+Proof.
+  have: forall a b, parallel a b -> lc_tm a /\ lc_tm b.
+  { intros a b P. induction P; split; split_hyp; eauto.
+  eapply lc_abs_open; eauto.
+  
+  pick fresh x. repeat spec x. split_hyp. eapply lc_abs_exists; eauto.
+  pick fresh x. repeat spec x. split_hyp. eapply lc_abs_exists; eauto. 
+  }
+  intros h.
+  split;  intros a b h1; edestruct h; eauto.
+Qed. 
+
+#[local]
+Instance parallel_reflexive : reflexive parallel.
+Proof.
+  constructor. intros t LC.
+  induction LC; eauto.
+  all: econstructor; try econstructor; eauto. 
+  Unshelve. exact empty.
+Qed.
+
+
+#[local]
+Instance subst1_parallel : substitutive parallel.
+Proof.
+  constructor. unfold subst1.
+  intros t t' x u LCu Vu Ptt'. 
+  induction Ptt'; simpl.
+  all: try eauto.
+  - (* beta *)
+    autorewrite with lngen; auto.
+  - (* var *)
+    destruct_var_eq;
+    eauto using reflexivity.
+  - (* abs *)
+    pick fresh y and apply p_abs.
+    spec y.
+    rewrite_subst_open_hyp.
+Qed.
+
+#[local]
+Instance compatible_parallel : compatible parallel.
+Proof.
+  split. 
+  + intros x t u Fr P.
+    pick fresh y and apply p_abs.
+    rewrite (subst_tm_intro x t); auto.
+    rewrite (subst_tm_intro x u); auto.
+    eapply subst; eauto. 
+  + intros. eauto using reflexivity.
+  + intros. eauto using reflexivity.
+  + intros. eauto using reflexivity.
+  + intros. eauto using reflexivity.
+
+Qed.
+
+(** ** Lemma 3.2.4  
+
+   Parallel reduction satisfies the second and third substitution properties.
+   This is a key part of the Church-Rosser proof.
+ *)
+
+(** This is done inline. But we have already identified this property for 
+   relations, so we'll prove it separately first. *)
+Lemma subst2_parallel : subst2 parallel.
+Proof.
+  unfold subst2.
+  intros x t u u' LC Vu P.
+  induction LC; simpl.
+  all: auto.
+  - (* var *)
+    destruct_var_eq; auto. 
+  - (* abs *)
+    pick fresh y and apply p_abs.
+    spec y.
+    rewrite_subst_open_hyp.
+    eapply lc1; eauto.
+    eapply parallel_reflexive.
+    eapply lc2; eauto. 
+Qed.
+
+(** Parallel reduction is *not* transitive. So we need to prove this by induction. *)
+Lemma subst3_parallel : subst3 parallel.
+Proof.
+  unfold subst3.
+  intros x t t' u u' Vu Vu' Ptt' Puu'.
+  have LCu : lc_tm u. { eapply lc1; eauto. }
+  have LCu' : lc_tm u'. { eapply lc2; eauto. }
+  induction Ptt'; simpl.
+  all: try move: (value_subst v x u' H Vu') => vh.
+  all: eauto.
+  - (* beta *)
+    autorewrite with lngen; auto.
+  - (* var *)
+    destruct_var_eq; auto.
+  - (* abs *)
+    pick fresh y and apply p_abs.
+    spec y.
+    rewrite_subst_open_hyp.
+Qed.
+
+(** A corollary of the above lets us reason about parallel reduction for opened terms. *)
+Corollary parallel_open : forall x t t' u u',
+  x `notin` fv_tm t 
+  -> x `notin` fv_tm t'
+  -> parallel (t ^ x) (t' ^ x) 
+  -> parallel u u' 
+  -> parallel (open t u) (open t' u').
+Proof.  
+  intros x t t' u u' F1 F2 H0 P41.
+Admitted.
+(*
+  move: (subst3_parallel x _ _ _ _ H0 P41) => h.
+  repeat rewrite subst_tm_open_tm_wrt_tm in h; eauto.
+  eapply lc1; eauto with lngen.
+  eapply lc2; eauto with lngen.
+  repeat rewrite subst_eq_var in h.
+  repeat rewrite subst_tm_fresh_eq in h; auto.
+Qed.
+*)
+
+
+(* ================================================================= *)
+
+(** ** Lemma 3.2.6 *)
+
+(** The first of our two key lemmas: parallel reduction satisfies 
+the diamond property. *)
+
+Lemma diamond_property_parallel : diamond_property parallel.
+Proof.
+  (* WORKED IN CLASS *)
+  unfold diamond_property.
+  intros t t1 t2 H1 H2.
+  move: t2 H2. (* make IH stronger *)
+  induction H1; 
+    intros t2 H2; inversion H2; subst.
+  - (* beta / beta *)
+Admitted.
+(*
+    destruct (IHparallel1 _ H1) as [t3' [P31 P32]].
+    inversion P31. subst.
+    inversion P32. subst.
+    destruct (IHparallel2 _ H4) as [t4' [P41 P42]].
+    pick fresh x. spec x.
+    exists (open t'1 t4'). 
+    split; eauto using parallel_open. 
+  - (* beta / app *)
+    destruct (IHparallel1 _ H1) as [t2 [P1 P2]].
+    inversion P1. subst.
+    destruct (IHparallel2 _ H4) as [t3 [P3 P4]].
+    pick fresh x. spec x.
+    exists (open t'1 t3).
+    split; eauto using parallel_open.
+  - (* var / var *)
+    exists (var_f x). split; auto.
+  - (* abs / abs *)
+    pick fresh x. repeat spec x.
+    destruct (H0 _ H3) as [t3 [P1 P2]].
+    exists (abs (close x t3)).
+    split.
+    eapply (compatible_abs x);
+    autorewrite with lngen; auto.
+    eapply (compatible_abs x);
+    autorewrite with lngen; auto.
+  - (* app / beta *)
+    destruct (IHparallel1 _ H1) as [t2 [P1 P2]].
+    inversion P2. subst.
+    destruct (IHparallel2 _ H4) as [t3 [P3 P4]].
+    pick fresh x. spec x.
+    exists (open t'1 t3).
+    split; eauto using parallel_open. 
+  - (* app / app *)
+    destruct (IHparallel1 _ H1) as [t2 [P1 P2]].
+    destruct (IHparallel2 _ H4) as [t3 [P3 P4]].
+    exists (app t2 t3).
+    split; auto.
+Qed. *)
+
+(* ================================================================= *)
+
+(** This next part talks about relations between relations. To make this 
+    a bit easier to work with, we'll introduce some notation for when 
+    one relation implies another and when one relation is equivalent to 
+    another
+*)
+
+Module RelationNotation.
+  Notation "R1 [<=] R2" := (forall t u, R1 t u -> R2 t u).
+  Notation "R1 [=] R2" := (forall t u, R1 t u <-> R2 t u).
+End RelationNotation.
+Import RelationNotation.
+
+(** ** Lemma 3.2.7 *)
+
+(** Lemma 3.2.7 states that 
+
+               beta_reduction = trans_closure parallel
+
+   To prove this lemma, Barendregt notes that 
+
+           refl_closure (compatible_closure beta) [<=] parallel [<=] beta_reduction
+
+   He then says: 
+
+      Since beta_reduction is the transitive closure of the first, then it is also 
+      the transitive closure of parallel reduction.
+
+  This proof is captured in then next four lemmas.
+
+*)
+
+
+(*
+Lemma refl_compatible_sub_parallel : refl_closure (compatible_closure beta) [<=] parallel.
+Proof.
+  intros t u H. dependent induction H.
+  - dependent induction H.
+    + inversion H. eapply p_beta; eauto using reflexivity.
+    + pick fresh x. spec x. eapply (compatible_abs x); eauto.
+    + eapply compatible_app1; eauto using reflexivity.
+    + eapply compatible_app2; eauto using reflexivity.      
+  - eapply reflexivity; auto.
+Qed.
+
+(** *** Exercise [parallel_sub_beta_reduction] *)
+
+Lemma parallel_sub_beta_reduction : parallel [<=] beta_reduction.
+Proof. (* FILL IN HERE *) Admitted.
+
+Lemma beta_reduction_trans_refl_cc : beta_reduction [=] trans_closure (refl_closure (compatible_closure beta)).
+Proof.
+  unfold beta_reduction, R_reduction in *. 
+  split; intros h; dependent induction h; eauto.
+  inversion H. eauto. eapply reflexivity. auto.
+Qed.
+
+Lemma  beta_reduction_is_trans_closure_parallel : 
+   beta_reduction [=] trans_closure parallel.
+Proof. 
+  intros.
+  split.
+  - rewrite beta_reduction_trans_refl_cc.
+    (* relies on R1 [<=] R2 implies trans_closure R1 [<=] trans_closure R2
+       where R1 is refl_closure (cc beta) and R2 is parallel reduction 
+     *)
+    intros h.
+    dependent induction h.
+    eapply t_rel. 
+    eapply refl_compatible_sub_parallel. auto.
+    eapply t_trans; eauto.
+  - intros h.
+    (* relies on R1 [<=] R2 implies trans_closure R1 [<=] trans_closure R2
+       where R1 is parallel reduction and R2 is beta_reduction. 
+       Also observe: trans_closure (beta_reduction) [=] beta_reduction *)
+    dependent induction h.
+    eapply parallel_sub_beta_reduction; auto. 
+    eapply transitivity; eauto.
+Qed.
+
+(** To use this result, we also need to show that the diamond
+    property respects relational equivalence. This is mostly a matter 
+    of unfolding definitions. *)
+
+Lemma diamond_respects : forall R1 R2,
+  R1 [=] R2 ->
+  diamond_property R1 ->
+  diamond_property R2.
+Proof.
+  intros R1 R2 rr.
+  unfold diamond_property. 
+  intros db t1 t2 t3 T1 T2.
+  rewrite <- rr in T1.
+  rewrite <- rr in T2.
+  destruct (db t1 t2 t3 T1 T2) as [t4 [b1 b2]].
+  exists t4.
+  rewrite -> rr in b1.
+  rewrite -> rr in b2.
+  split; auto.
+Qed.
+
+(* ================================================================= *)
+
+(** * Lemma 3.2.8 (Church-Rosser Theorem) *)
+
+Lemma church_rosser_beta : church_rosser beta.
+Proof.
+  unfold church_rosser.
+  fold beta_reduction.
+  eapply diamond_respects.
+  symmetry.
+  eapply beta_reduction_is_trans_closure_parallel.
+  apply diamond_property_trans_closure.
+  apply diamond_property_parallel.
+Qed.
+
+(* ================================================================= *)
+
+(** ** Corollary 3.2.9 (i) *)
+
+Lemma nf_reduce_beta : forall u t, R_nf_of beta u t -> beta_reduction t u.
+Proof.
+  intros. eapply nf_reduce; eauto.
+  typeclasses eauto.
+  eapply church_rosser_beta.
+Qed.
+
+(** ** Corollary 3.2.9 (ii) *)
+
+Lemma nf_unique_beta : forall u1 u2 t, R_nf_of beta u1 t -> R_nf_of beta u2 t -> u1 = u2.
+Proof.
+  intros u1 u2 t h1 h2. 
+  move: (nf_reduce_beta _ _ h1) => r1.
+  move: (nf_reduce_beta _ _ h2) => r2.
+  destruct h1 as [h1 h1'].
+  destruct h2 as [h2 h2'].
+  move: (church_rosser_beta _ _ _ r1 r2) => [v [r1' r2']].
+  apply nf_noreduction in r1'; auto. destruct r1' as [eq nfv1]. subst.
+  apply nf_noreduction in r2'; auto. destruct r2' as [eq nfv2]. subst.
+  auto.
+Qed.
+
+Lemma joinability t u (H : beta_convertibility t u) :
+  exists v, beta_reduction t v /\ beta_reduction u v.
+Proof.
+  apply convertibility_reduction_diamond.
+  apply church_rosser_beta.
+  auto.
+Qed.
+
+(** ** Main result: different normal forms are not beta convertible. *)
+
+Lemma consistency : forall t u, nf beta t -> nf beta u -> t <> u -> not (beta_convertibility t u).
+Proof.
+  intros.
+  intros h.
+  move: (joinability _ _ h) => [v [rtv ruv]].
+  move: (nf_noreduction _ H _ rtv) => [EQ nfv].
+  move: (nf_noreduction _ H0 _ ruv) => [EQ' nfv'].
+  rewrite <- EQ' in EQ.
+  contradiction.
+Qed.
+
+
+(** For completness, we will exhibit two different normal forms. *)
+
+(* " \x. \y. x" *)
+Definition church_true := abs (abs (var_b 1)).
+
+(* " \x. \y. y" *)
+Definition church_false := abs (abs (var_b 0)).
+
+Lemma nf_true : nf beta church_true.
+Proof.
+  pick fresh x and apply nf_abs.
+  pick fresh y and apply nf_abs.
+  apply nf_var.
+  intro h; inversion h; inversion H.
+  intro h; inversion h; inversion H.
+  intro h; inversion h; inversion H.
+Qed.
+
+Lemma nf_false : nf beta church_false.
+Proof.
+  pick fresh x and apply nf_abs.
+  pick fresh y and apply nf_abs.
+  apply nf_var.
+  intro h; inversion h; inversion H.
+  intro h; inversion h; inversion H.
+  intro h; inversion h; inversion H.
+Qed.
+
+Lemma not_convertible_true_false : not (beta_convertibility church_true church_false).
+Proof.
+  apply consistency.
+  apply nf_true.
+  apply nf_false.
+  intro h. inversion h.
+Qed.
+*)
